kami-rv32im: fixed the program init. not to make any back pressure.

Kami/PrimBram.v
@@ -2,24 +2,44 @@ Require Import Arith.Peano_dec Bool String List.
 Require Import Lib.Word Lib.Indexer.
 Require Import Kami.Syntax Kami.Notations Kami.Semantics.
 Require Import Kami.Wf Kami.Tactics.
-Require Import Kami.PrimFifo.
 
 Set Implicit Arguments.
+
+Definition isSomeB {A} (a: option A) :=
+  match a with
+  | Some _ => true
+  | None => false
+  end.
+
+Definition isNoneB {A} (a: option A) :=
+  match a with
+  | Some _ => false
+  | None => true
+  end.
+
+Definition optionVal {ty dType} (ov: option (ty dType)):
+  Expr ty (SyntaxKind dType) :=
+  match ov with
+  | Some v => (#v)%kami_expr
+  | None => ($$Default)%kami_expr
+  end.
+
+Definition liftSome {A} (a: A): option A :=
+  Some a.
 
 Definition primBramName: string := "BRAM".
 
 Section PrimBram.
   Variables (bramName: string)
-            (outFIFODepth: nat)
             (addrSize: nat)
             (dType: Kind).
 
   Local Notation "^ s" := (bramName -- s) (at level 0).
 
-  Definition bramRssT ty := list (ty dType).
-  Definition bramRssK ty := @NativeKind (bramRssT ty) nil.
-  Definition bramRss ty :=
-    (^"rss" :: (@NativeConst (bramRssT ty) nil nil))%struct.
+  Definition bramReadValT (ty: Kind -> Type) := option (ty dType).
+  Definition bramReadValK ty := @NativeKind (bramReadValT ty) None.
+  Definition bramReadVal ty :=
+    (^"rss" :: (@NativeConst (bramReadValT ty) None None))%struct.
 
   Definition BramRq :=
     STRUCT {
@@ -31,33 +51,32 @@ Section PrimBram.
   Definition bramPutRq: forall ty (rq: ty (Struct BramRq)), ActionT ty Void :=
     fun ty rq =>
       (Read bram <- ^"bram";
-       ReadN rss: bramRssK ty <- ^"rss";
-       Assert !$$(listIsFull outFIFODepth rss);
        If #rq!BramRq@."write" then
          LET writev <- #rq!BramRq@."datain";
          Write ^"bram" <- #bram@[#rq!BramRq@."addr" <- #writev];
-         Write ^"rss" <- (Var _ (bramRssK ty) (listEnq writev rss));
          Retv
        else
-         LET readv <- #bram@[#rq!BramRq@."addr"];
-         Write ^"rss" <- (Var _ (bramRssK ty) (listEnq readv rss));
+         ReadN readVal: bramReadValK ty <- ^"readVal";
+         Assert $$(isNoneB readVal);
+         LET readv: dType <- #bram@[#rq!BramRq@."addr"];
+         Write ^"readVal" <- Var _ (bramReadValK ty) (liftSome readv);
          Retv;
        Retv)%kami_action.
 
   Definition bramGetRs: forall ty (_: ty Void), ActionT ty dType :=
     fun ty _ =>
-      (ReadN rss: bramRssK ty <- ^"rss";
-       Assert !$$(listIsEmpty rss);
-       Write ^"rss" <- (Var _ (bramRssK ty) (listDeq rss));
-       Ret (listFirstElt rss))%kami_action.
+      (ReadN readVal: bramReadValK ty <- ^"readVal";
+       Assert $$(isSomeB readVal);
+       Write ^"readVal" <- (Var _ (bramReadValK ty) None);
+       Ret (optionVal readVal)%kami_action)%kami_action.
   
   Definition bram1: Modules :=
     PrimMod
       {| pm_name := primBramName;
          pm_regInits :=
            [(^"bram" :: (RegInitDefault (SyntaxKind (Vector dType addrSize))))%struct;
-              (^"rss" :: (RegInitCustom (existT ConstFullT (bramRssK type)
-                                                (NativeConst nil nil))))%struct];
+              (^"readVal" :: (RegInitCustom (existT ConstFullT (bramReadValK type)
+                                                    (NativeConst None None))))%struct];
          pm_rules := nil;
          pm_methods :=
            [(^"putRq" :: (existT _ {| arg:= _; ret:= _ |} bramPutRq))%struct;
@@ -68,24 +87,23 @@ End PrimBram.
 
 Hint Unfold bram1 : ModuleDefs.
 Hint Unfold primBramName
-     bramRssT bramRssK bramRss
+     bramReadValT bramReadValK bramReadVal
      BramRq bramPutRq bramGetRs: MethDefs.
 
 Section Facts.
   Variables (bramName: string)
-            (outFIFODepth: nat)
             (addrSize: nat)
             (dType: Kind).
 
   Lemma bram1_ModEquiv:
-    ModPhoasWf (bram1 bramName outFIFODepth addrSize dType).
+    ModPhoasWf (bram1 bramName addrSize dType).
   Proof.
     kequiv.
   Qed.
   Hint Resolve bram1_ModEquiv.
 
   Lemma bram1_ValidRegs:
-    ModRegsWf (bram1 bramName outFIFODepth addrSize dType).
+    ModRegsWf (bram1 bramName addrSize dType).
   Proof.
     kvr.
   Qed.
